added kset map to value relation

TwoSortHet/Term.lean
@@ -1,23 +1,156 @@
 
+import TwoSortHet.Util
 import LeanSubst
-import TwoSortHet.Ty
+open LeanSubst
 
 namespace TwoSortHet
 
-open LeanSubst
+----------------------------------------------------------------------------------------------------
+-- Syntax
+----------------------------------------------------------------------------------------------------
 
-inductive Term : Type where
+inductive Kind where
+| base : Kind
+
+notation "★" => Kind.base
+--infixr:64 " -:> " => Kind.arrow
+
+inductive Ty where
+| var : Nat -> Ty
+--| app : Ty -> Ty -> Ty
+--| lam : Kind -> Ty -> Ty
+| all : Kind -> Ty -> Ty
+| arrow : Ty -> Ty -> Ty
+
+prefix:max "t#" => Ty.var
+infixr:64 " -:> " => Ty.arrow
+--notation "λ[" K "]" t => Ty.lam K t
+notation "∀[" K "]" B => Ty.all K B
+--infixl:54 " • " => Ty.app
+
+inductive Term where
 | var : Nat -> Term
 | app : Term -> Term -> Term
-| tapp : Term -> Ty -> Term
 | lam : Ty -> Term -> Term
-| tlam : Term -> Term
+| tapp : Term -> Ty -> Term
+| tlam : Kind -> Term -> Term
 
 prefix:max "#" => Term.var
-notation:65 f:65 " :@ " a:64 => Term.app f a
-notation:65 f:65 " :@[" a "]" => Term.tapp f a
-notation ":λ[" A "] " t => Term.lam A t
-notation "Λ " t => Term.tlam t
+notation "λ[" A "]" t => Term.lam A t
+notation "Λ[" K "]" B => Term.tlam K B
+infixl:54 " • " => Term.app
+notation f " •[" a "]" => Term.tapp f a
+
+----------------------------------------------------------------------------------------------------
+-- Substitution of Ty
+----------------------------------------------------------------------------------------------------
+
+@[coe]
+def Ty.from_action : Subst.Action Ty -> Ty
+| .re y => t#y
+| .su t => t
+
+@[simp]
+theorem Ty.from_action_id {n} : from_action (+0.act n) = t#n := by
+  simp [from_action, Subst.id]
+
+@[simp]
+theorem Ty.from_action_succ {n} : from_action (+1.act n) = t#(n + 1) := by
+  simp [from_action, Subst.succ]
+
+@[simp]
+theorem Ty.from_acton_re {n} : from_action (re n) = t#n := by simp [from_action]
+
+@[simp]
+theorem Ty.from_action_su {t} : from_action (su t) = t := by simp [from_action]
+
+instance : Coe (Subst.Action Ty) Ty where
+  coe := Ty.from_action
+
+@[simp]
+def Ty.rmap (r : Ren) : Ty -> Ty
+| t#x => t#(r.act x)
+| A -:> B => rmap r A -:> rmap r B
+| ∀[K] P => ∀[K] rmap r.lift P
+-- | λ[K] t => λ[K] rmap r.lift t
+-- | app f a => rmap r f • rmap r a
+
+instance : RenMap Ty where
+  rmap := Ty.rmap
+
+@[simp]
+theorem Ty.ren_var : (t#x)⟨r⟩ = t#(r.act x) := by simp [RenMap.rmap]
+
+@[simp]
+theorem Ty.ren_arr {A B : Ty} : (A -:> B)⟨r⟩ = A⟨r⟩ -:> B⟨r⟩ := by simp [RenMap.rmap]
+
+@[simp]
+theorem Ty.ren_all : (∀[K] P)⟨r⟩ = ∀[K] P⟨r.lift⟩ := by simp [RenMap.rmap]
+
+-- @[simp]
+-- theorem Ty.ren_lam {P : Ty} : (λ[K] P)⟨r⟩ = λ[K] P⟨r.lift⟩ := by simp [RenMap.rmap]
+
+-- @[simp]
+-- theorem Ty.ren_app {f a : Ty} : (f • a)⟨r⟩ = f⟨r⟩ • a⟨r⟩ := by simp [RenMap.rmap]
+
+instance : RenMapId Ty where
+  apply_id := by subst_solve_id
+
+instance : RenMapCompose Ty where
+  apply_compose := by subst_solve_compose
+
+@[simp]
+def Ty.smap (σ : Subst Ty) : Ty -> Ty
+| t#x => σ.act x
+| A -:> B => smap σ A -:> smap σ B
+| ∀[K] P => ∀[K] smap σ.lift P
+-- | λ[K] t => λ[K] smap σ.lift t
+--| app f a => smap σ f • smap σ a
+
+instance : SubstMap Ty Ty where
+  smap := Ty.smap
+
+@[simp]
+theorem Ty.subst_var : (t#x)[σ:Ty] = σ.act x := by simp [SubstMap.smap]
+
+@[simp]
+theorem Ty.subst_arr {A B : Ty} : (A -:> B)[σ:Ty] = A[σ:_] -:> B[σ:_] := by simp [SubstMap.smap]
+
+@[simp]
+theorem Ty.subst_all : (∀[K] P)[σ:Ty] = ∀[K] P[σ.lift:_] := by simp [SubstMap.smap]
+
+-- @[simp]
+-- theorem Ty.subst_lam {P : Ty} : (λ[K] P)[σ:Ty] = λ[K] P[σ.lift:_] := by simp [SubstMap.smap]
+
+-- @[simp]
+-- theorem Ty.subst_app {f a : Ty} : (f • a)[σ:Ty] = f[σ:_] • a[σ:_] := by simp [SubstMap.smap]
+
+@[simp]
+theorem Ty.from_action_compose {x} {σ τ : Subst Ty}
+  : (from_action (σ.act x))[τ] = from_action ((σ ∘ τ).act x)
+:= by
+  simp [Ty.from_action, Subst.compose]
+  generalize zdef : σ.act x = z
+  cases z <;> simp [Ty.from_action]
+
+instance : SubstMapId Ty Ty where
+  apply_id := by subst_solve_id
+
+instance : SubstMapStable Ty where
+  apply_stable := by subst_solve_stable
+
+instance : SubstMapRenComposeLeft Ty Ty where
+  apply_ren_compose_left := by subst_solve_compose
+
+instance : SubstMapRenComposeRight Ty Ty where
+  apply_ren_compose_right := by subst_solve_compose
+
+instance : SubstMapCompose Ty Ty where
+  apply_compose := by subst_solve_compose
+
+----------------------------------------------------------------------------------------------------
+-- Substitution of Term
+----------------------------------------------------------------------------------------------------
 
 @[coe]
 def Term.from_action : Subst.Action Term -> Term
@@ -25,11 +158,11 @@ def Term.from_action : Subst.Action Term -> Term
 | .su t => t
 
 @[simp]
-theorem Term.from_action_id {n} : from_action (+0 n) = #n := by
+theorem Term.from_action_id {n} : from_action (+0.act n) = #n := by
   simp [from_action, Subst.id]
 
 @[simp]
-theorem Term.from_action_succ {n} : from_action (+1 n) = #(n + 1) := by
+theorem Term.from_action_succ {n} : from_action (+1.act n) = #(n + 1) := by
   simp [from_action, Subst.succ]
 
 @[simp]
@@ -42,143 +175,174 @@ instance : Coe (Subst.Action Term) Term where
   coe := Term.from_action
 
 @[simp]
-def Term.rmap (lf : Endo Ren) (r : Ren) : Term -> Term
-| #x => #(r x)
-| f :@ a => rmap lf r f :@ rmap lf r a
-| f :@[a] => rmap lf r f :@[a]
-| :λ[A] t => :λ[A] rmap lf (lf r) t
-| Λ t => Λ rmap lf r t
+def Term.Ty.rmap (r : HetRen Ty) : Term -> Term
+| #x => #x
+| λ[A] t => λ[A⟨r.forget⟩] rmap r t
+| Λ[K] t => Λ[K] rmap r.lift t
+| app f a => rmap r f • rmap r a
+| f •[a] => rmap r f •[a⟨r.forget⟩]
+
+instance : HetRenMap Term Ty where
+  hrmap := Term.Ty.rmap
+
+@[simp]
+theorem Term.Ty.ren_var {r : HetRen Ty} : (#x)⟨r⟩ = #x := by simp [HetRenMap.hrmap]
+
+@[simp]
+theorem Term.Ty.ren_lam {r : HetRen Ty} {t : Term} : (λ[A] t)⟨r⟩ = λ[A⟨r.forget⟩] t⟨r⟩ := by simp [HetRenMap.hrmap]
+
+@[simp]
+theorem Term.Ty.ren_tlam {r : HetRen Ty} {t : Term} : (Λ[K] t)⟨r⟩ = Λ[K] t⟨r.lift⟩ := by simp [HetRenMap.hrmap]
+
+@[simp]
+theorem Term.Ty.ren_app {r : HetRen Ty} {f a : Term} : (f • a)⟨r⟩ = f⟨r⟩ • a⟨r⟩ := by simp [HetRenMap.hrmap]
+
+@[simp]
+theorem Term.Ty.ren_tapp {r : HetRen Ty} {f : Term} : (f •[a])⟨r⟩ = f⟨r⟩ •[a⟨r.forget⟩] := by simp [HetRenMap.hrmap]
+
+instance : HetRenMapId Term Ty where
+  apply_id := by subst_solve_id
+
+instance : HetRenMapCompose Term Ty where
+  apply_compose := by subst_solve_compose
+
+@[simp]
+def Term.rmap (r : Ren) : Term -> Term
+| #x => #(r.act x)
+| λ[A] t => λ[A] rmap r.lift t
+| Λ[K] t => Λ[K] rmap r t
+| app f a => rmap r f • rmap r a
+| f •[a] => rmap r f •[a]
 
 instance : RenMap Term where
   rmap := Term.rmap
 
 @[simp]
-def Term.Ty.smap (lf : Endo (Subst Ty)) (σ : Subst Ty) : Term -> Term
+theorem Term.ren_var : (#x)⟨r⟩ = #(r.act x) := by simp [RenMap.rmap]
+
+@[simp]
+theorem Term.ren_lam {t : Term} : (λ[A] t)⟨r⟩ = λ[A] t⟨r.lift⟩ := by simp [RenMap.rmap]
+
+@[simp]
+theorem Term.ren_tlam {t : Term} : (Λ[K] t)⟨r⟩ = Λ[K] t⟨r⟩ := by simp [RenMap.rmap]
+
+@[simp]
+theorem Term.ren_app {f a : Term} : (f • a)⟨r⟩ = f⟨r⟩ • a⟨r⟩ := by simp [RenMap.rmap]
+
+@[simp]
+theorem Term.ren_tapp {f : Term} : (f •[a])⟨r⟩ = f⟨r⟩ •[a] := by simp [RenMap.rmap]
+
+instance : RenMapId Term where
+  apply_id := by subst_solve_id
+
+instance : RenMapCompose Term where
+  apply_compose := by subst_solve_compose
+
+@[simp]
+def Term.Ty.smap (σ : Subst Ty) : Term -> Term
 | #x => #x
-| f :@ a => smap lf σ f :@ smap lf σ a
-| f :@[a] => smap lf σ f :@[a[σ]]
-| :λ[A] t => :λ[A[σ]] smap lf σ t
-| Λ t => Λ smap lf (lf σ) t
+| λ[A] t => λ[A[σ:_]] smap σ t
+| Λ[K] t => Λ[K] smap σ.lift t
+| app f a => smap σ f • smap σ a
+| f •[a] => smap σ f •[a[σ:_]]
 
 instance : SubstMap Term Ty where
   smap := Term.Ty.smap
 
 @[simp]
-def Term.smap (lf : Endo (Subst Term)) (σ : Subst Term) : Term -> Term
-| #x => σ x
-| f :@ a => smap lf σ f :@ smap lf σ a
-| f :@[a] => smap lf σ f :@[a]
-| :λ[A] t => :λ[A] smap lf (lf σ) t
-| Λ t => Λ smap lf (σ ◾ +1@Ty) t
+def Term.smap (σ : Subst Term) : Term -> Term
+| #x => σ.act x
+| λ[A] t => λ[A] smap σ.lift t
+| Λ[K] t => Λ[K] smap (σ ◾ +1@Ty) t
+| app f a => smap σ f • smap σ a
+| f •[a] => smap σ f •[a]
 
 instance : SubstMap Term Term where
   smap := Term.smap
 
 @[simp]
-theorem Term.subst_var : (#x)[σ:Term] = σ x := by
-  unfold Subst.apply; simp [SubstMap.smap]
+theorem Term.Ty.subst_var : (#x)[σ:Ty] = #x := by simp [SubstMap.smap]
 
 @[simp]
-theorem Term.subst_app : (f :@ a)[σ:Term] = f[σ:_] :@ a[σ:_] := by
-  unfold Subst.apply; simp [SubstMap.smap]
+theorem Term.Ty.subst_lam {t : Term} : (λ[A] t)[σ:Ty] = λ[A[σ:_]] t[σ:_] := by simp [SubstMap.smap]
 
 @[simp]
-theorem Term.subst_tapp : (f :@[a])[σ:Term] = f[σ:_] :@[a] := by
-  unfold Subst.apply; simp [SubstMap.smap]
+theorem Term.Ty.subst_tlam : (Λ[K] t)[σ:Ty] = Λ[K] t[σ.lift:_] := by simp [SubstMap.smap]
 
 @[simp]
-theorem Term.subst_lam : (:λ[A] t)[σ:Term] = :λ[A] t[σ.lift:_] := by
-  unfold Subst.apply; simp [SubstMap.smap]
+theorem Term.Ty.subst_app {f a : Term} : (f • a)[σ:Ty] = f[σ:_] • a[σ:_] := by simp [SubstMap.smap]
 
 @[simp]
-theorem Term.subst_tlam : (Λ t)[σ:Term] = Λ t[σ ◾ +1@Ty:_] := by
-  unfold Subst.apply; simp [SubstMap.smap]
+theorem Term.Ty.subst_tapp : (f •[a])[σ:Ty] = f[σ:_] •[a[σ:_]] := by simp [SubstMap.smap]
+
+@[simp]
+theorem Term.subst_var : (#x)[σ:Term] = σ.act x := by simp [SubstMap.smap]
+
+@[simp]
+theorem Term.subst_lam {t : Term} : (λ[A] t)[σ:Term] = λ[A] t[σ.lift:_] := by simp [SubstMap.smap]
+
+@[simp]
+theorem Term.subst_tlam : (Λ[K] t)[σ:Term] = Λ[K] t[σ ◾ +1@Ty:_] := by simp [SubstMap.smap]
+
+@[simp]
+theorem Term.subst_app {f a : Term} : (f • a)[σ:Term] = f[σ:_] • a[σ:_] := by simp [SubstMap.smap]
+
+@[simp]
+theorem Term.subst_tapp : (f •[a])[σ:Term] = f[σ:_] •[a] := by simp [SubstMap.smap]
 
 @[simp]
 theorem Term.from_action_compose {x} {σ τ : Subst Term}
-  : (from_action (σ x))[τ] = from_action ((σ ∘ τ) x)
+  : (from_action (σ.act x))[τ] = from_action ((σ ∘ τ).act x)
 := by
   simp [Term.from_action, Subst.compose]
-  generalize zdef : σ x = z
+  generalize zdef : σ.act x = z
   cases z <;> simp [Term.from_action]
 
 @[simp]
-theorem Term.Ty.subst_var : (#x)[σ:Ty] = #x := by
-  simp [Subst.apply, SubstMap.smap]
-
-@[simp]
-theorem Term.Ty.subst_app : (f :@ a)[σ:Ty] = f[σ:_] :@ a[σ:_] := by
-  simp [Subst.apply, SubstMap.smap]
-
-@[simp]
-theorem Term.Ty.subst_tapp : (f :@[a])[σ:Ty] = f[σ:_] :@[a[σ:Ty]] := by
-  simp [Subst.apply, SubstMap.smap]
-
-@[simp]
-theorem Term.Ty.subst_lam : (:λ[A] t)[σ:Ty] = :λ[A[σ:Ty]] t[σ:_] := by
-  simp [Subst.apply, SubstMap.smap]
-
-@[simp]
-theorem Term.Ty.subst_tlam : (Λ t)[σ:Ty] = Λ t[σ.lift:_] := by
-  simp [Subst.apply, SubstMap.smap]
-
-theorem Term.Ty.apply_id {t : Term} : t[+0:Ty] = t := by
-  induction t
-  all_goals (simp at * <;> try simp [*])
-
-instance : SubstMapId Term Ty where
-  apply_id := Term.Ty.apply_id
-
-@[simp]
 theorem Term.hcompose_var {σ : Subst Term} {τ : Subst Ty}
-  : (σ ◾ τ) x = (Term.from_action (σ x))[τ:Ty]
+  : (σ ◾ τ).act x = (Term.from_action (σ.act x))[τ:Ty]
 := by
   simp [Subst.hcompose, Term.from_action]
-  generalize zdef : σ x = z
+  generalize zdef : σ.act x = z
   cases z <;> simp
 
-theorem Term.apply_stable (r : Ren) (σ : Subst Term)
-  : r.to = σ -> Ren.apply (T := Term) r = Subst.apply σ
-:= by subst_solve_stable Term, r, σ
+instance : SubstMapId Term Ty where
+  apply_id := by subst_solve_id
 
 instance : SubstMapStable Term where
-  apply_stable := Term.apply_stable
+  apply_stable := by subst_solve_stable
 
 theorem Term.apply_ren_commute {s : Term} (r : Ren) (τ : Subst Ty)
-  : s[r.to][τ:Ty] = s[τ:Ty][r.to]
+  : s⟨r⟩[τ:Ty] = s[τ:Ty]⟨r⟩
 := by
-  induction s generalizing r τ <;> simp [Ren.to] at *
+  induction s generalizing r τ <;> simp at *
   all_goals try simp [*]
-  case lam A t ih =>
-    replace ih := ih r.lift
-    rw [Ren.to_lift (S := Term)] at ih; simp at ih
-    apply ih
 
 instance : SubstMapRenCommute Term Ty where
   apply_ren_commute := Term.apply_ren_commute
 
-theorem Term.Ty.apply_compose {s : Term} {σ τ : Subst Ty} : s[σ:Ty][τ:_] = s[σ ∘ τ:_] := by
-  subst_solve_compose Ty, s, σ, τ
+instance : SubstMapRenComposeLeft Term Ty where
+  apply_ren_compose_left := by subst_solve_compose
+
+instance : SubstMapRenComposeRight Term Ty where
+  apply_ren_compose_right := by subst_solve_compose
 
 instance : SubstMapCompose Term Ty where
-  apply_compose := Term.Ty.apply_compose
-
-theorem Term.apply_hcompose {s : Term} {σ : Subst Term} {τ : Subst Ty}
-  : s[σ][τ:_] = s[τ:_][σ ◾ τ]
-:= by subst_solve_hcompose Term, Ty, s, σ, τ
-
-instance : SubstMapHetCompose Term Ty where
-  apply_hcompose := Term.apply_hcompose
-
-theorem Term.apply_id {t : Term} : t[+0] = t := by subst_solve_id Term, Ty, t
+  apply_compose := by subst_solve_compose
 
 instance : SubstMapId Term Term where
-  apply_id := Term.apply_id
+  apply_id := by subst_solve_id
 
-theorem Term.apply_compose {s : Term} {σ τ : Subst Term} : s[σ][τ] = s[σ ∘ τ] := by
-  subst_solve_compose Term, s, σ, τ
+instance : SubstMapHetCompose Term Ty where
+  apply_hcompose := by subst_solve_compose
+
+instance : SubstMapRenComposeLeft Term Term where
+  apply_ren_compose_left := by subst_solve_compose
+
+instance : SubstMapRenComposeRight Term Term where
+  apply_ren_compose_right := by subst_solve_compose
 
 instance : SubstMapCompose Term Term where
-  apply_compose := Term.apply_compose
+  apply_compose := by subst_solve_compose
 
 end TwoSortHet
