TwoSortHet/Kinding/Rename.lean
@@ -1,0 +1,30 @@
+
+import TwoSortHet.Typing
+open LeanSubst
+
+namespace TwoSortHet
+
+structure KindingRen (r : Ren) (Δ1 Δ2 : List Kind) where
+  act : ∀ {x T}, Δ1[x]? = some T -> Δ2[r.act x]? = some T
+
+notation:35 Γ:35 " -⟨" r "⟩> " Δ:35 => KindingRen r Γ Δ
+
+theorem KindingRen.lift A : Δ1 -⟨r⟩> Δ2 -> A::Δ1 -⟨r.lift⟩> A::Δ2 := λ h => .mk (λ {x} {_} h2 => match x with
+  | 0 => h2
+  | _ + 1 => h.act h2)
+
+theorem KindingRen.id X : X -⟨.id⟩> X := .mk (λ h => h)
+
+theorem KindingRen.succ : X -⟨Ren.add 1⟩> A::X := .mk (λ h => h)
+
+theorem KindingRen.comp : A -⟨r1⟩> B -> B -⟨r2⟩> C -> A -⟨r1 ∘ r2⟩> C := λ h1 h2 => .mk
+  λ h3 => sorry
+
+def Kinding.rename (m : Δ1 -⟨r⟩> Δ2) : Δ1 ⊢ₖ A : K -> Δ2 ⊢ₖ A⟨r⟩ : K
+| var h => var (m.act h)
+-- | lam j => lam (j.rename $ m.lift _)
+--| app j1 j2 => app (j1.rename m) (j2.rename m)
+| all j => all (j.rename $ m.lift _)
+| arrow j1 j2 => arrow (j1.rename m) (j2.rename m)
+
+end TwoSortHet
