TwoSortHet/Kinding/StrongNorm.lean
@@ -1,0 +1,170 @@
+
+import LeanSubst
+import TwoSortHet.Typing
+import TwoSortHet.Kinding.Substitute
+open LeanSubst
+
+namespace TwoSortHet
+
+def KSet := List Kind -> Ty -> Kind -> Prop
+def KSet.empty : KSet := λ _ _ _ => False
+def KRed := List Kind -> Ty -> Ty -> Prop
+
+def ℛₖ (S : List Kind -> Ty -> Prop) : List Kind -> Ty -> Prop
+| Δ1, t => ∀ {r Δ2}, Δ1 -⟨r⟩> Δ2 -> S Δ2 t[r]
+
+mutual
+  inductive Kinding.SnNor : (List Kind -> Ty -> Prop) -> KSet
+  -- | lam :
+  --   ℛₖ S1 Δ (λ[A] t) ->
+  --   SnNor S2 (A::Δ) t B ->
+  --   SnNor S1 Δ (λ[A] t) (A -:> B)
+  | all :
+    SnNor S (A::Δ) t ★ ->
+    SnNor S Δ (∀[A] t) ★
+  | arrow :
+    SnNor S Δ A ★ ->
+    SnNor S Δ B ★ ->
+    SnNor S Δ (A -:> B) ★
+  | neu :
+    SnNeu S Δ A K ->
+    SnNor S Δ A K
+  -- | red :
+  --   SnRed Δ S A A' ->
+  --   SnNor Δ S A' K ->
+  --   SnNor Δ S A K
+
+  inductive Kinding.SnNeu : (List Kind -> Ty -> Prop) -> KSet
+  | var :
+    Δ[x]? = some K ->
+    SnNeu S Δ t#x K
+  -- | app :
+  --   SnNeu S1 Δ f (A -:> B) ->
+  --   SnNor S2 Δ a A ->
+  --   SnNeu S3 Δ (f • a) B
+
+  -- inductive Kinding.SnRed : (List Kind -> Ty -> Prop) -> KRed
+  -- | beta :
+  --   SnNor S1 Δ t A ->
+  --   Δ ⊢ₖ λ[A] b : (A -:> B) ->
+  --   SnRed S2 Δ ((λ[A] b) • t) b[su t::+0]
+  -- | app :
+  --   SnRed S1 Δ f f' ->
+  --   SnRed S2 Δ (f • a) (f' • a)
+end
+
+mutual
+  theorem Kinding.SnNor.soundness : SnNor S Δ A K -> Δ ⊢ₖ A : K
+  --| .lam h1 h2 => Kinding.lam (Kinding.SnNor.soundness h2)
+  | .all h1 => Kinding.all (Kinding.SnNor.soundness h1)
+  | .arrow h1 h2 => Kinding.arrow (Kinding.SnNor.soundness h1) (Kinding.SnNor.soundness h2)
+  | .neu h1 => Kinding.SnNeu.soundness h1
+  --| .red h1 h2 => Kinding.SnRed.soundness h1 (Kinding.SnNor.soundness h2)
+
+  theorem Kinding.SnNeu.soundness : SnNeu S Δ A K -> Δ ⊢ₖ A : K
+  | .var h1 => Kinding.var h1
+  -- | .app h1 h2 => Kinding.app (Kinding.SnNeu.soundness h1) (Kinding.SnNor.soundness h2)
+
+  -- theorem Kinding.SnRed.soundness : SnRed S Δ A A' -> Δ ⊢ₖ A' : K -> Δ ⊢ₖ A : K
+  -- | .beta h1 (.lam h2), j1 =>
+  --   let lem := Kinding.beta h2 (Kinding.SnNor.soundness h1)
+  --   let lem2 := Kinding.unique j1 lem
+  --   Kinding.app (.lam h2) (Kinding.SnNor.soundness h1) |> cast (by rw [lem2])
+  -- | .app h1, Kinding.app j1 j2 => Kinding.app (Kinding.SnRed.soundness h1 j1) j2
+end
+
+mutual
+  theorem Kinding.SnNor.rename (m : Δ1 -⟨r⟩> Δ2) : SnNor S Δ1 A K -> SnNor S Δ2 A[r] K
+  -- | SnNor.lam (S2 := S2) (t := t) (A := A) (B := B) f th =>
+
+  --   Kinding.SnNor.lam (S2 := S2) (t := t[r.to.lift]) (λ m' => f (.comp m m') |> cast (by simp)) (th.rename (m.lift A) |> cast (by rw [Ren.to_lift]))
+  | .all (A := A) (t := t) h =>
+    SnNor.all (h.rename (KindingRen.lift A m)) |> cast (by rw [Ren.to_lift]; simp)
+  | .arrow h1 h2 => .arrow (h1.rename m) (h2.rename m)
+  | .neu h => .neu (h.rename m)
+  -- | .red h1 h2 => .red (h1.rename m) (h2.rename m)
+
+  theorem Kinding.SnNeu.rename (m : Δ1 -⟨r⟩> Δ2) : SnNeu S Δ1 A K -> SnNeu S Δ2 A[r] K
+  | .var h => .var (m.act h)
+  -- | .app h1 h2 => .app (h1.rename m) (h2.rename m)
+
+  -- theorem Kinding.SnRed.rename (m : Δ1 -⟨r⟩> Δ2) : SnRed S Δ1 A B -> SnRed S Δ2 A[r] B[r]
+  -- | .beta (S1 := S1) (t := t) (A := A) (b := b) h j => by
+  --   have lem1 := (Kinding.subst (KindingRen.to m) j)
+  --   simp at lem1
+  --   have lem := SnRed.beta (S2 := S) (b := b[.re 0 :: r ∘ +1]) (.rename m h) lem1
+  --   simp at *
+  --   apply lem
+  -- | .app h => .app (h.rename m)
+end
+
+@[simp]
+def 𝒱ₖ : Kind -> List Kind -> Ty -> Prop
+--| A -:> B, Δ, λ[_] t => ∀ {a}, Kinding.SnNor (𝒱ₖ A) Δ a A -> Kinding.SnNor (𝒱ₖ B) Δ t[su a::+0] B
+| _, _, _ => False
+
+structure Kinding.SemSubst (Δ1 Δ2 : List Kind) (σ : Subst Ty) where
+  act : ∀ {i T}, Δ1[i]? = some T -> SnNor (𝒱ₖ T) Δ2 (σ.act i) T
+
+notation:35 Γ:35 " -⟦" σ "⟧> " Δ:35 => Kinding.SemSubst Γ Δ σ
+
+theorem Kinding.SemSubst.id : Δ -⟦+0⟧> Δ := .mk (λ h => SnNor.neu (SnNeu.var h))
+
+theorem Kinding.SemSubst.lift (m : Γ -⟦σ⟧> Δ) A : A::Γ -⟦σ.lift⟧> A::Δ := SemSubst.mk @λ i _ h =>
+  match i with
+  | 0 => SnNor.neu (SnNeu.var h)
+  | _ + 1 => by
+    simp_all
+    have e1 := m.act h
+    have lem := SnNor.rename (Δ2 := A :: Δ) (KindingRen.succ (X := Δ)) e1
+    simp at lem
+    apply lem
+
+theorem Kinding.SemSubst.compose (m1 : Γ -⟦σ⟧> Δ) (m2 : Δ -⟨r⟩> Ξ) : Γ -⟦σ ∘ r.to⟧> Ξ := SemSubst.mk @λ i _ h =>
+  have e2 := m1.act h
+  SnNor.rename m2 e2 |> cast (by simp)
+
+theorem Kinding.SemSubst.su (j : SnNor (𝒱ₖ A) Δ a A) (m : Γ -⟦σ⟧> Δ) : A::Γ -⟦su a::σ⟧> Δ := SemSubst.mk @ λ i _ h =>
+  match i with
+  | 0 => by simp_all
+  | _ + 1 => m.act h
+
+@[simp]
+def SemanticKinding (Δ1 : List Kind) (A : Ty) (K : Kind) :=
+  ∀ {σ Δ2}, Δ1 -⟦σ⟧> Δ2 -> Kinding.SnNor (𝒱ₖ K) Δ2 A[σ] K
+
+notation:170 Γ:170 " ⊨ₖ " t:170 " : " A:170 => SemanticKinding Γ t A
+
+-- theorem Kinding.app_induction:
+--   S = 𝒱ₖ (A -:> K) ->
+--   T = A -:> K ->
+--   SnNor S Δ2 f T ->
+--   SnNor (𝒱ₖ A) Δ2 a A ->
+--   SnNor (𝒱ₖ K) Δ2 (f • a) K
+-- | eq1, eq2, SnNor.lam (t := t) h1 h2, j2 =>
+--   let lem2 : (λ x => x) = @id Nat := by unfold id; rfl
+--   let lem : SnNor (𝒱ₖ K) Δ2 t[su a :: +0] K := by
+--     subst eq1
+--     simp [ℛₖ] at h1
+--     replace h1 := h1 (KindingRen.id Δ2) j2
+--     apply h1
+--   have lem3 := Kinding.SnNor.soundness h2
+--   SnNor.red (SnRed.beta (by simp at eq2; rcases eq2 with ⟨e1,e2⟩; rw [<-e1]at j2; apply j2) (Kinding.lam lem3)) lem
+-- | eq1, eq2, .neu h, j2 => by subst eq1 eq2; apply SnNor.neu (SnNeu.app h j2)
+-- | eq1, eq2, .red h1 h2, j2 => SnNor.red (SnRed.app h1) (Kinding.app_induction eq1 eq2 h2 j2)
+
+theorem Kinding.fundamental : Δ ⊢ₖ A : K -> Δ ⊨ₖ A : K
+| var j, σ, Δ2, h => h.act j
+-- | lam (A := A) (t := t) (B := B) j, σ, Δ2, h =>
+--   let j' : (A :: Δ) ⊨ₖ t : B := fundamental j
+--   have lem {Δ2' r} : Δ2 -⟨r⟩> Δ2' → 𝒱ₖ (A -:> B) Δ2' (λ[A] t[σ.lift][r.to.lift]) := λ j1 T j2 =>
+--     j' (SemSubst.su (a := T) j2 (SemSubst.compose h j1)) |> cast (by simp)
+--   SnNor.lam (t := t[σ.lift]) lem (j' (SemSubst.lift h A))
+-- | app j1 j2, σ, Δ2, h =>
+--   let j1' := fundamental j1 h
+--   let j2' := fundamental j2 h
+--   Kinding.app_induction rfl rfl j1' j2'
+| all j, σ, Δ2, h => .all $ j.fundamental $ h.lift _
+| arrow j1 j2, σ, Δ2, h => .arrow (j1.fundamental h) (j2.fundamental h)
+
+end TwoSortHet
