TwoSortHet/Kinding/Substitute.lean
@@ -1,0 +1,66 @@
+
+import TwoSortHet.Typing
+import TwoSortHet.Kinding.Rename
+open LeanSubst
+
+namespace TwoSortHet
+
+structure KindingSubst (σ : Subst Ty) (Δ1 Δ2 : List Kind) where
+  act : ∀ {x T}, Δ1[x]? = some T -> Δ2 ⊢ₖ σ.act x : T
+
+notation:35 Γ:35 " -[" σ "]> " Δ:35 => KindingSubst σ Γ Δ
+
+theorem KindingSubst.id Δ : Δ -[+0]> Δ := KindingSubst.mk λ h => .var h
+
+theorem KindingSubst.re (j : Δ2[y]? = some A) (m : Δ1 -[σ]> Δ2) : A::Δ1 -[re y::σ]> Δ2 := KindingSubst.mk λ h => sorry
+
+theorem KindingSubst.su (j : Δ2 ⊢ₖ a : A) (m : Δ1 -[σ]> Δ2) : A::Δ1 -[su a::σ]> Δ2 := sorry
+
+theorem KindingSubst.lift A :
+  Δ1 -[σ]> Δ2 ->
+  A::Δ1 -[σ.lift]> A::Δ2
+:= sorry
+
+theorem KindingSubst.succ A : Δ -[+1]> A::Δ := sorry
+
+theorem KindingSubst.comp : A -[σ]> B -> B -[τ]> C -> A -[σ ∘ τ]> C := sorry
+
+theorem KindingRen.to (m : A -⟨r⟩> B) : A -[r.to]> B := sorry
+
+theorem Kinding.subst (m : Δ1 -[σ]> Δ2) : Δ1 ⊢ₖ A : K -> Δ2 ⊢ₖ A[σ] : K
+| var h => m.act h
+-- | lam j => lam (j.subst $ m.lift _)
+-- | app j1 j2 => app (j1.subst m) (j2.subst m)
+| all j => all (j.subst $ m.lift _)
+| arrow j1 j2 => arrow (j1.subst m) (j2.subst m)
+
+theorem Kinding.beta : (A::Δ) ⊢ₖ b : B -> Δ ⊢ₖ t : A -> Δ ⊢ₖ b[su t::+0] : B
+| j1, j2 => subst (.su j2 $ .id _) j1
+
+-- theorem Kinding.preservation_step : Δ ⊢ₖ A : K -> A ~t> A' -> Δ ⊢ₖ A' : K
+-- | .lam (A := A) h1, .lam_congr j1 => .lam (Kinding.preservation_step h1 j1)
+-- | .app h1 h2, .app_congr1 j1 => .app (Kinding.preservation_step h1 j1) h2
+-- | .app h1 h2, .app_congr2 j1 => .app h1 (Kinding.preservation_step h2 j1)
+-- | .all h1, .all_congr j1 => .all (Kinding.preservation_step h1 j1)
+-- | .arrow h1 h2, .arrow_congr1 j1 => .arrow (Kinding.preservation_step h1 j1) h2
+-- | .arrow h1 h2, .arrow_congr2 j1 => .arrow h1 (Kinding.preservation_step h2 j1)
+-- | .app (.lam h1) h2, .beta => Kinding.beta h1 h2
+
+-- theorem regularity : Δ&Γ ⊢ t : A -> Δ ⊢ₖ A : ★
+-- | .var h1 h2 => h2
+-- | .lam h1 h2 =>
+--   .arrow h1 (regularity h2)
+-- | .app h1 h2 =>
+--   let lem := regularity h1
+--   match lem with
+--   |.arrow j1 j2 => j2
+-- | .tlam h1 =>
+--   let lem := regularity h1
+--   .all lem
+-- | .tapp h1 h2 h3 =>
+--   let lem := regularity h1
+--   match lem with
+--   | .all j1 => Kinding.beta j1 h2 |> cast (by rw [h3])
+-- | .conv (A := A) (B := B) h1 h2 h3 => h3
+
+end TwoSortHet
