TwoSortHet/Kinding/Value.lean
@@ -1,0 +1,75 @@
+import LeanSubst
+import TwoSortHet.Typing
+import TwoSortHet.Kinding.Substitute
+open LeanSubst
+
+namespace TwoSortHet
+
+-- inductive Neutral : Ty -> Prop where
+-- | var : Neutral (.var x)
+-- | app : Neutral f -> Neutral (f • a)
+
+-- inductive Value : Ty -> Prop where
+-- | var : Value (.var x)
+-- | arrow : Value A -> Value B -> Value (A -:> B)
+-- | lam : Value t -> Value (λ[K] t)
+-- | all : Value t -> Value (∀[K] t)
+-- | app : Neutral f -> Value f -> Value a -> Value (f • a)
+
+-- theorem var_step : t#x ~t> A -> ∃ y, A = t#y
+-- | j1 => by cases j1
+
+-- theorem var_star_step : t#x ~t>* A -> ∃ y, A = t#y
+-- | .refl => ⟨x, rfl⟩
+-- | .step h1 h2 =>
+--   let ⟨y', e1⟩ := var_star_step h1
+--   by
+--     rw [e1] at h2
+--     replace h2 := var_step h2
+--     apply h2
+
+-- theorem app_neutral_step : Neutral f -> f ~t> y -> Neutral y
+-- | .app h1, .app_congr1 j1 => .app (app_neutral_step h1 j1)
+-- | .app h1, .app_congr2 j1 => .app h1
+
+-- theorem app_neutral_star_step : Neutral f -> f ~t>* y -> Neutral y
+-- | j1, .refl => j1
+-- | j1, .step h1 h2 => app_neutral_step (app_neutral_star_step j1 h1) h2
+
+-- --need confluence
+-- theorem Typing.unique : Δ&Γ ⊢ t : A -> Δ&Γ ⊢ t : A' -> A =t= A'
+-- | .var h1 h2, .var j1 j2 => by rw [h1] at j1; injection j1 with w; subst w; apply Conv.refl
+-- | .var h1 h2, .conv j1 j2 j3 =>
+--   let lem := Typing.unique (.var h1 h2) j1
+--   sorry
+-- | .lam h1 h2, .lam j1 j2 =>
+--   sorry
+-- | .lam h1 h2, .conv j1 j2 j3 =>
+--   let lem := Typing.unique (.lam h1 h2) j1
+--   sorry
+-- | .app h1 h2, .app j1 j2 => sorry
+-- | .app h1 h2, .conv j1 j2 j3 =>
+--   let lem := Typing.unique (.app h1 h2) j1
+--   sorry
+-- | .tlam h1, .tlam j1 => sorry
+-- | .tlam h1, .conv j1 j2 j3 =>
+--   let lem := Typing.unique (.tlam h1) j1
+--   sorry
+-- | .tapp h1 h2 h3, .tapp j1 j2 j3 => sorry
+-- | .tapp h1 h2 h3, .conv j1 j2 j3 =>
+--   let lem := Typing.unique (.tapp h1 h2 h3) j1
+--   sorry
+-- | .conv h1 h2 h3, .var j1 j2 =>
+--   --let lem := Typing.unique h1 j1
+--   sorry
+-- | .conv h1 h2 h3, .lam j1 j2 => sorry
+-- | .conv h1 h2 h3, .app j1 j2 => sorry
+-- | .conv h1 h2 h3, .tlam j1 => sorry
+-- | .conv h1 h2 h3, .tapp j1 j2 j3 =>
+--   --let lem := Typing.unique h1 (.tapp j1 j2 j3)
+--   sorry
+-- | .conv h1 h2 h3, .conv j1 j2 j3 =>
+--   let lem := Typing.unique h1 j1
+--   sorry
+
+end TwoSortHet
