TwoSortHet/Typing.lean
@@ -1,0 +1,97 @@
+
+import LeanSubst
+import TwoSortHet.Term
+import TwoSortHet.Reduction
+open LeanSubst
+
+namespace TwoSortHet
+
+inductive Kinding : List Kind -> Ty -> Kind -> Prop where
+| var :
+  Δ[x]? = some K ->
+  Kinding Δ t#x K
+-- | lam :
+--   Kinding (A::Δ) t B ->
+--   Kinding Δ (λ[A] t) (A -:> B)
+-- | app :
+--   Kinding Δ f (A -:> B) ->
+--   Kinding Δ a A ->
+--   Kinding Δ (f • a) B
+| all :
+  Kinding (K::Δ) P ★ ->
+  Kinding Δ (∀[K] P) ★
+| arrow :
+  Kinding Δ A ★ ->
+  Kinding Δ B ★ ->
+  Kinding Δ (A -:> B) ★
+
+notation:170 Δ:170 " ⊢ₖ " A:170 " : " K:170 => Kinding Δ A K
+
+inductive Typing : List Kind -> List Ty -> Term -> Ty -> Prop where
+| var :
+  Γ[x]? = some T ->
+  Δ ⊢ₖ T : ★ ->
+  Typing Δ Γ #x T
+| lam :
+  Δ ⊢ₖ A : ★ ->
+  Typing Δ (A::Γ) t B ->
+  Typing Δ Γ (λ[A] t) (A -:> B)
+| app :
+  Typing Δ Γ f (A -:> B) ->
+  Typing Δ Γ a A ->
+  Typing Δ Γ (f • a) B
+| tlam :
+  Typing (K::Δ) Γ⟨.add 1⟩ t P ->
+  Typing Δ Γ (Λ[K] t) (∀[K] P)
+| tapp :
+  Typing Δ Γ f (∀[K] P) ->
+  Δ ⊢ₖ a : K ->
+  P' = P[su a::+0] ->
+  Typing Δ Γ (f •[a]) P'
+-- | conv :
+--   Typing Δ Γ t A ->
+--   A =t= B ->
+--   Δ ⊢ₖ B : ★ ->
+--   Typing Δ Γ t B
+
+notation:170 Δ:170 "&" Γ:170 " ⊢ " t:170 " : " A:170 => Typing Δ Γ t A
+
+-- theorem Typing.type_preservation : Δ&Γ ⊢ t : A -> Δ ⊢ₖ A' : ★ -> A ~t> A' -> Δ&Γ ⊢ t : A'
+-- | h1, j1, j2 => .conv h1 (.backward .refl j2) j1
+
+-- theorem test : A =t= A' -> (A -:> B) =t= (A' -:> B)
+-- | .refl => .refl
+-- | .forward h1 h2 =>
+--   let lem := test (B := B) h1
+--   let lem2 := Ty.Red.arrow_congr1 (B := B) h2
+--   let lem3 := Conv.forward lem lem2
+--   lem3
+-- | .backward h1 h2 =>
+--   let lem := test (B := B) h1
+--   let lem2 := Ty.Red.arrow_congr1 (B := B) h2
+--   Conv.backward lem lem2
+
+-- -- | .refl, j1 => j1
+-- -- | .backward (y := A'') h1 h2, j1 =>
+-- --   let lem := Ty.Red.arrow_congr1 (B := B) h2
+-- --   have lem2 : Δ&Γ ⊢ t : (A'' -:> B) := type_preservation j1 sorry lem
+-- --   .arrow_congr1 h1 lem2
+-- -- | .forward (x := A'') h1 h2, j1 =>
+-- --   let lem := Ty.Red.arrow_congr1 (B := B) h2
+-- --   sorry
+
+-- theorem Typing.arrow_congr2 : B =t= B' -> Δ&Γ ⊢ t : (A -:> B') -> Δ&Γ ⊢ t : (A -:> B') := sorry
+
+-- theorem Kinding.unique : Δ ⊢ₖ A : K -> Δ ⊢ₖ A : K' -> K = K'
+-- | .var h1, .var j1 => by rw [h1] at j1; injection j1
+-- | .lam h1, .lam j1 =>
+--   let lem := Kinding.unique h1 j1
+--   by rw [lem]
+-- | .app h1 h2, .app j1 j2 =>
+--   let lem1 := Kinding.unique h1 j1
+--   let lem2 := Kinding.unique h2 j2
+--   by rw [lem2] at h1; injection lem1
+-- | .all h1, .all j1 => rfl
+-- | .arrow h1 h2, .arrow j1 j2 => rfl
+
+end TwoSortHet
