TwoSortHet/Typing/Rename.lean
@@ -1,0 +1,79 @@
+
+import TwoSortHet.Typing
+import TwoSortHet.Kinding.Rename
+import TwoSortHet.Kinding.Substitute
+open LeanSubst
+
+namespace TwoSortHet
+
+structure TypingRen (r : Ren) (Γ1 Γ2 : List Ty) where
+  act : ∀ {x T}, Γ1[x]? = some T -> Γ2[r.act x]? = some T
+
+notation:35 Γ:35 " -⟨" r "⟩> " Δ:35 => TypingRen r Γ Δ
+
+theorem TypingRen.lift {Γ1 Γ2 : List Ty} A : Γ1 -⟨r⟩> Γ2 -> A::Γ1 -⟨r.lift⟩> A::Γ2
+| j => .mk @λ x T h =>
+  match x with
+  | 0 => by simp at *; subst h; rfl
+  | n + 1 =>
+    have lem := j.act h
+    by simp [Ren.lift] at *; apply lem
+
+theorem TypingRen.rename {Γ1 : List Ty} k : {Γ2 : List Ty} -> Γ1 -⟨r⟩> Γ2 -> Γ1⟨k⟩ -⟨r⟩> Γ2⟨k⟩
+| .nil, ⟨a⟩ => mk λ {x T} h => by
+  simp at *
+  rw [List.rmap_to_map] at h; simp at h
+  rcases h with ⟨q, h1, h2⟩
+  subst h2; apply a h1
+| .cons hd Γ2, m => mk λ {x T} h => by
+  simp
+  rw [List.rmap_to_map] at h; simp at h
+  rcases h with ⟨q, h1, h2⟩; subst h2
+  have lem := m.act h1
+  generalize zdef : r.act x = z at *
+  cases z <;> simp at *; subst lem; rfl
+  case _ z =>
+    have lem2 : Γ2⟨k⟩[z]? = (some q)⟨k⟩ := by rw [<-lem]; simp
+    simp at lem2; exact lem2
+
+theorem TypingRen.id (X : List Ty) : X -⟨.id⟩> X := .mk λ h => h
+
+theorem TypingRen.succ {X : List Ty} : X -⟨Ren.add 1⟩> A::X := .mk λ h => h
+
+theorem TypingRen.comp {A B C : List Ty} : A -⟨r1⟩> B -> B -⟨r2⟩> C -> A -⟨r1 ∘ r2⟩> C
+| h1, h2 => .mk λ h =>
+  have lem1 := h1.act h
+  have lem2 := h2.act lem1
+  lem2
+
+def Typing.rename_type {Δ1 Δ2 : List Kind} (m : Δ1 -⟨r⟩> Δ2)
+  : Δ1&Γ ⊢ t : A -> Δ2&Γ⟨r⟩ ⊢ t⟨r.het Ty⟩ : A⟨r⟩
+| var (x := x) h j =>
+  let h' : Γ⟨r⟩[x]? = (some A)⟨r⟩ := by rw [<-h]; simp
+  var h' (j.rename m)
+| lam j1 j2 => lam (j1.rename m) (j2.rename_type m)
+| app j1 j2 => app (j1.rename_type m) (j2.rename_type m)
+| tlam j =>
+  let j' := j.rename_type $ m.lift _
+  tlam $ j' |> cast (by sorry)
+| tapp (P := P) (a := a) j1 j2 e =>
+  let e' : A⟨r⟩ = P⟨r.lift⟩[su a⟨r⟩ :: +0] := by
+    simp [e]
+    rw [Subst.apply_stable r.lift r.to.lift Ren.to_lift]
+    rw [Subst.apply_stable r _ rfl]
+    simp
+  tapp (P := P⟨r.lift⟩) (j1.rename_type m) (j2.rename m) e'
+--| conv j1 cv j2 => sorry
+
+def Typing.rename {Γ1 Γ2 : List Ty} (m : Γ1 -⟨r⟩> Γ2)
+  : Δ&Γ1 ⊢ t : A -> Δ&Γ2 ⊢ t⟨r⟩ : A
+| var h j => var (m.act h) j
+| lam j1 j2 => lam j1 $ j2.rename (m.lift _)
+| app j1 j2 => app (j1.rename m) (j2.rename m)
+| tlam j => tlam $ j.rename $ m.rename (Ren.add 1)
+| tapp j1 j2 e => tapp (j1.rename m) j2 e
+--| conv j1 cv j2 => sorry
+
+#check (#0)[su #1 :: su #0 :: +0]
+
+end TwoSortHet
