TwoSortHet/Typing/StrongNorm.lean
@@ -1,0 +1,291 @@
+
+import LeanSubst
+import TwoSortHet.Typing
+import TwoSortHet.Typing.Substitute
+import TwoSortHet.Kinding.StrongNorm
+import TwoSortHet.Kinding.Value
+import TwoSortHet.Reduction
+open LeanSubst
+
+namespace TwoSortHet
+
+def TSet := List Kind -> List Ty -> Term -> Ty -> Prop
+def TSet.empty : TSet := λ _ _ _ _ => False
+def TRed := List Kind -> List Ty -> Term -> Term -> Ty -> Prop
+
+def LR := List Kind -> List Ty -> Term -> Prop
+--(A : Ty) -> (Nat -> KSet) -> (Δ : List Kind) -> (Γ : List Ty) -> (t : Term) ->  Prop
+
+def ℛ (S : LR) : LR
+| Δ, Γ1, t => ∀ {r Γ2}, Γ1 -⟨r⟩> Γ2 -> S Δ Γ2 t[r]
+
+mutual
+  inductive Typing.SnNor : LR -> TSet
+  | lam :
+    --Kinding.SnNor S Δ A K -> Value (A -:> B) ->
+    ℛ S1 Δ Γ (λ[A] t) ->
+    SnNor S2 Δ (A::Γ) t B ->
+    Δ ⊢ₖ A : ★ ->
+    SnNor S1 Δ Γ (λ[A] t) (A -:> B)
+  | tlam :
+    ℛ S1 Δ Γ (Λ[K] t) ->
+    SnNor S2 (K::Δ) Γ⟨.add 1⟩ t P ->
+    SnNor S1 Δ Γ (Λ[K] t) (∀[K] P)
+  | neu :
+    SnNeu S Δ Γ t A ->
+    SnNor S Δ Γ t A
+  | red :
+    SnRed S2 Δ Γ t t' A ->
+    SnNor S Δ Γ t' A ->
+    SnNor S Δ Γ t A
+
+  inductive Typing.SnNeu : LR -> TSet
+  | var :
+    Γ[x]? = some A ->
+    Δ ⊢ₖ A : ★ ->
+    SnNeu S Δ Γ #x A
+  | app :
+    SnNeu S1 Δ Γ f (A -:> B) ->
+    SnNor S2 Δ Γ a A ->
+    SnNeu S3 Δ Γ (f • a) B
+  | tapp :
+    SnNeu S1 Δ Γ f (∀[K] P) ->
+    P' = P[su a::+0] ->
+    Kinding.SnNor S2 Δ a K ->
+    SnNeu S3 Δ Γ (f •[a]) P'
+
+  inductive Typing.SnRed : LR -> TRed
+  | beta :
+    SnNor S1 Δ Γ t A ->
+    Δ&Γ ⊢ (λ[A]b) : (A -:> B) ->
+    SnRed S2 Δ Γ ((λ[A] b) • t) b[su t::+0] B
+  | tbeta :
+    Δ ⊢ₖ t : K ->
+    Δ&Γ ⊢ (Λ[K] b) : (∀[K] P) ->
+    P' = P[su t::+0] ->
+    SnRed S Δ Γ ((Λ[K] b) •[t]) b[su t::+0:Ty] P'
+  | app :
+    Δ&Γ ⊢ a : A ->
+    SnRed S1 Δ Γ f f' (A -:> B) ->
+    Δ&Γ ⊢ f' : (A -:> B) ->
+    SnRed S2 Δ Γ (f • a) (f' • a) B
+  | tapp :
+    Δ ⊢ₖ a : K ->
+    SnRed S1 Δ Γ f f' (∀[K] P) ->
+    Δ&Γ ⊢ f' : (∀[K] P) ->
+    P' = P[su a::+0] ->
+    SnRed S2 Δ Γ (f •[a]) (f' •[a]) P'
+end
+
+mutual
+  theorem Typing.SnNor.rename {Γ1 Γ2 : List Ty} (m : Γ1 -⟨r⟩> Γ2)
+    : SnNor S Δ Γ1 t A -> SnNor S Δ Γ2 t[r] A
+  | Typing.SnNor.lam h1 h2 h3 => by simp; sorry
+  | .tlam h1 h2 => sorry
+  | .neu h1 => SnNor.neu (Typing.SnNeu.rename m h1)
+  | .red h2 h3  => SnNor.red (SnRed.rename m h2) (.rename m h3)
+
+  theorem Typing.SnNeu.rename {Γ1 Γ2 : List Ty} (m : Γ1 -⟨r⟩> Γ2)
+    : SnNeu S Δ Γ1 t A -> SnNeu S Δ Γ2 t[r] A := sorry
+
+  theorem Typing.SnRed.rename {Γ1 Γ2 : List Ty} (m : Γ1 -⟨r⟩> Γ2)
+    : SnRed S Δ Γ1 t t' A -> SnRed S Δ Γ2 t[r] t'[r] A
+  | .beta h1 h2 => sorry
+  | .tbeta h1 h2 h3 => sorry
+  | .app h1 h2 h3 => sorry
+  | .tapp h1 h2 h3 h4 => sorry
+end
+
+def KSetcons : KSet -> (Nat -> KSet) -> (Nat -> KSet)
+| K, _, 0 => K
+| _, ξ, n + 1 => ξ n
+
+
+@[simp]
+def KSet.int_term (v : Nat -> KSet) : Ty -> KSet
+| t#x => v x
+| P -:> Q => A (int_term v P) (int_term v Q)
+| ∀[K] t => Q (λ d => int_term (d::v) t)
+
+@[simp]
+def Model.int_subst (v : Nat -> KSet) (σ : Subst Ty) : Nat -> KSet
+| i => KSet.int_term v (σ.act i)
+
+@[simp]
+def 𝒱 : (A : Ty) -> (Nat -> KSet) -> (Δ : List Kind) -> (Γ : List Ty) -> (t : Term) ->  Prop
+| A -:> B, ξ, Δ, Γ, λ[_] t => ∀ {a}, Typing.SnNor (𝒱 A ξ) Δ Γ a A -> Typing.SnNor (𝒱 B ξ) Δ Γ t[su a::+0] B
+| ∀[K] P, ξ, Δ, Γ, Λ[_] t  => ∀ {a : Ty}, Kinding.SnNor (𝒱ₖ K) Δ a K -> Typing.SnNor (𝒱 P (KSetcons (Kinding.SnNor (𝒱ₖ K)) ξ)) Δ Γ t[su a::+0:Ty] P[su a::+0:Ty] --added
+--| t#x, ξ, Δ, _, _ => ξ x Δ (t#x) ★ disgusting
+| _, _, _, _, _ => False
+
+structure Typing.SemSubst (Δ : List Kind) (Γ1 Γ2 : List Ty) (σ : Subst Term) (ξ : (Nat -> KSet)) where
+  act : ∀ {i T}, Γ1[i]? = some T -> (SnNor (𝒱 T ξ) Δ Γ2 (σ.act i) T)
+
+notation:160 Δ:170 " ⊢ " Γ1:170 " -⟦" σ ";" ξ "⟧> " Γ2:170 => Typing.SemSubst Δ Γ1 Γ2 σ ξ
+
+-- theorem Typing.arrow_congr1 : Δ ⊢ₖ A' : ★ -> A =t= A' -> Δ&Γ ⊢ t : (A -:> B) -> Δ&Γ ⊢ t : (A' -:> B)
+-- | h, j1, j2 =>
+--   let lem := regularity j2=
+--   match lem with
+--   | Kinding.arrow _ h2 => .conv j2 (test j1) (Kinding.arrow h h2)
+
+mutual
+  theorem Typing.SnNor.soundness : SnNor S Δ Γ t A -> Δ&Γ ⊢ t : A
+  | .lam _ h4 h5 => Typing.lam h5 (Typing.SnNor.soundness h4)
+  | .tlam h1 h2 => Typing.tlam (Typing.SnNor.soundness h2)
+  | .neu h2 => Typing.SnNeu.soundness h2
+  | .red h2 h3 => SnRed.soundness h2 (SnNor.soundness h3)
+
+  theorem Typing.SnNeu.soundness : SnNeu S Δ Γ t A -> Δ&Γ ⊢ t : A
+  | .var h1 h3 => Typing.var h1 h3
+  | .app h3 h4 => Typing.app (Typing.SnNeu.soundness h3) (Typing.SnNor.soundness h4)
+  | .tapp h2 h3 h4 => Typing.tapp (Typing.SnNeu.soundness h2) (Kinding.SnNor.soundness h4) h3
+
+  theorem Typing.SnRed.soundness : SnRed S Δ Γ t t' A -> Δ&Γ ⊢ t' : A -> Δ&Γ ⊢ t : A
+  | .beta h2 h3, j1 => Typing.app h3 (SnNor.soundness h2)
+  | .tbeta h2 h3 h4, j1 => Typing.tapp h3 h2 h4
+  | .app h1 h2 h3, Typing.app j1 j2 =>
+    let lem3 := SnRed.soundness h2 h3
+    Typing.app lem3 h1
+  | .tapp h1 h2 h3 h4, Typing.tapp _ j2 j3 => Typing.tapp (SnRed.soundness h2 h3) h1 h4
+end
+
+theorem Typing.SemSubst.id : Δ ⊢ X -⟦+0;ξ⟧> X := .mk @λ i T h1 => SnNor.neu (SnNeu.var h1 sorry)
+
+theorem Typing.SemSubst.lift (m : Δ ⊢ Γ1 -⟦σ;ξ⟧> Γ2) A : Δ ⊢ (A::Γ1) -⟦σ.lift;ξ⟧> (A::Γ2) := .mk @λ i T h1 =>
+  match i with
+  | 0 => SnNor.neu (SnNeu.var h1 sorry)
+  | n + 1 => by simp at *; sorry
+
+theorem Typing.SemSubst.compose (m1 : Δ ⊢ Γ1 -⟦σ;ξ⟧> Γ2) (m2 : Γ2 -⟨r⟩> Γ3)
+  : Δ ⊢ Γ1 -⟦σ ∘ r.to;ξ⟧> Γ3 := .mk @λ i T h1 => sorry
+
+theorem Typing.SemSubst.hcompose :
+  Δ1 ⊢ A -⟦σ;ξ⟧> B ->
+  Δ1 -⟨r⟩> Δ2 ->
+  Δ2 ⊢ A⟨r⟩ -⟦σ ◾ @r.to Ty;ξ⟧> B⟨r⟩
+:= sorry
+
+theorem Typing.SemSubst.su (j : SnNor (𝒱 A ξ) Δ Γ a A) (m : Δ ⊢ Γ1 -⟦σ;ξ⟧> Γ2) : Δ ⊢ (A::Γ1) -⟦su a::σ;ξ⟧> Γ2 := SemSubst.mk @ λ i _ h =>
+  sorry
+
+@[simp]
+def SemanticTyping (Δ : List Kind) (Γ1 : List Ty) (t : Term) (A : Ty) :=
+  ∀ {σ Γ2 ξ}, Δ ⊢ Γ1 -⟦σ;ξ⟧> Γ2 -> Typing.SnNor (𝒱 A ξ) Δ Γ2 t[σ] A
+
+notation:170 Δ:170 "&" Γ:170 " ⊨ " t:170 " : " A:170 => SemanticTyping Δ Γ t A
+
+theorem test :
+  Kinding.SnNor (𝒱ₖ K) Δ a K ->
+  Typing.SnNor (𝒱 P (KSetcons (Kinding.SnNor (𝒱ₖ K)) ξ)) Δ Γ t A->
+  Typing.SnNor (𝒱 P[su a :: +0] ξ) Δ Γ t A
+:= by sorry
+
+theorem SemanticTyping.tapp :
+  V = 𝒱 (∀[K] P) ξ ->
+  T = (∀[K] P) ->
+  Δ&Γ ⊢ f : T ->
+  Typing.SnNor V Δ Γ f T ->
+  Δ ⊢ₖ a : K ->
+  Kinding.SnNor (𝒱ₖ K) Δ a K ->
+  Typing.SnNor (𝒱 P[su a :: +0] ξ) Δ Γ (f •[a]) P[su a ::+0]
+| eq1, eq2, .tlam (t := t) j1, Typing.SnNor.tlam (S2 := S2) h1 h2, j3, j4 =>
+  by
+    injection eq2 with e1 e2
+
+    simp only [ℛ] at h1
+    symm at e1 e2
+    subst eq1 e1 e2
+    let h' : 𝒱 (∀[K]P) ξ Δ Γ (Λ[K]t)[.id] := h1 (TypingRen.id Γ)
+    simp at h'
+    replace h' := @h' a j4 --(𝒱 P[su a ::+0:Ty])
+    apply Typing.SnNor.red; apply Typing.SnRed.tbeta; apply j3; apply Typing.tlam j1; rfl; have lem := @test K Δ a P ξ Γ t[su a :: +0:_];
+    apply lem; apply j4; apply h'; apply S2 --apply h'; apply 𝒱 P[su a :: +0]
+| eq1, eq2, j1, .red (S2 := S2) (t' := f') h2 h3, j3, j4 =>
+  by
+    apply Typing.SnNor.red;
+    apply Typing.SnRed.tapp;
+    apply j3; rw [<-eq2] at *;
+    apply h2;
+    rw [<-eq2] at *; apply Typing.SnNor.soundness h3;
+    apply rfl;
+    apply SemanticTyping.tapp
+    apply eq1;
+    apply eq2;
+    apply Typing.SnNor.soundness h3; apply h3; apply j3; apply j4; apply S2;
+| eq1, eq2, j1, .neu h1, j3, j4 => Typing.SnNor.neu (Typing.SnNeu.tapp (h1 |> cast (by rw [<-eq2])) rfl j4)
+
+theorem SemanticTyping.app :
+  S = 𝒱 (A -:> B) ξ ->
+  T = A -:> B ->
+  Typing.SnNor S Δ Γ f T ->
+  Typing.SnNor (𝒱 A ξ) Δ Γ a A ->
+  Typing.SnNor (𝒱 B ξ) Δ Γ (f • a) B
+| eq1, eq2, Typing.SnNor.lam (t := t) (S2 := S2) h1 h2 h3, j2 =>
+  let lem2 : (λ x => x) = @id Nat := by unfold id; rfl
+  let lem : Typing.SnNor (𝒱 B ξ) Δ Γ t[su a :: +0] B := by
+    subst eq1
+    simp [ℛ] at h1
+    replace h1 := h1 (TypingRen.id Γ) j2
+    apply h1
+  have lem3 := Typing.SnNor.soundness h2
+  by
+    injection eq2 with e1 e2
+    apply Typing.SnNor.red; apply Typing.SnRed.beta; subst e1; apply j2; subst e1; rw [e2] at lem3; apply Typing.lam h3 lem3; apply lem; apply S2
+    --apply Typing.SnNor.red (Typing.SnRed.beta sorry (Typing.lam h3 (lem3))) lem
+| eq1, eq2, .neu h, j2 => by subst eq1 eq2; apply Typing.SnNor.neu (Typing.SnNeu.app h j2)
+| eq1, eq2, .red (S2 := S2) h1 h2, j2 =>
+  have lem1 := SemanticTyping.app eq1 eq2 h2 j2
+  by
+    apply Typing.SnNor.red; apply Typing.SnRed.app; apply Typing.SnNor.soundness j2; rw [eq2] at h1; apply h1; rw [eq2] at h2; apply Typing.SnNor.soundness h2; apply lem1; apply S2
+
+theorem Typing.fundamental : Δ&Γ ⊢ t : A -> Δ&Γ ⊨ t : A
+| var j1 j2, σ, Γ2, ξ, h => h.act j1
+| lam (t := t) (A := A) (B := B) j1 j2, σ, Γ2, ξ, h =>
+  let j2' : Δ&(A::Γ) ⊨ t : B := fundamental j2
+  sorry
+  --let lem2 := j2' h
+  -- have lem {Γ2' r'} : Γ2 -⟨r'⟩> Γ2' → 𝒱 (A -:> B) Δ Γ2' (λ[A]t[σ.lift][r'.to.lift]) := λ r a j2 =>
+  --   j2' (SemSubst.su j2 (SemSubst.compose h r)) |> cast (by simp)
+  -- SnNor.lam sorry sorry (t := t[σ.lift]) lem (j2' (SemSubst.lift h A))
+| app j1 j2, σ, Γ2, ξ, h =>
+  let j1' := fundamental j1 h
+  let j2' := fundamental j2 h
+  SemanticTyping.app rfl rfl j1' j2'
+| tlam (K := K) j, σ, Γ2, ξ, h =>
+  let h' : (K :: Δ) ⊢ Γ⟨.add 1⟩ -⟦σ ◾ +1;ξ⟧> Γ2⟨.add 1⟩ := h.hcompose (Δ2 := K::Δ) .succ
+  let j3' := j.fundamental h'
+  .tlam sorry j3'
+| tapp (a := a) (f := f) (K := K) (P := P) j1 j2 e, σ, Γ2, ξ, h =>
+  let lem := j1.fundamental h
+  let lem2 := j2.fundamental Kinding.SemSubst.id
+  by rw [e]; apply SemanticTyping.tapp; sorry; sorry; sorry; apply lem; apply j2; simp at lem2; apply lem2
+
+-- theorem Typing.SnNeu.consistency_lemma :
+--   Γ = [] ->
+--   SnNeu T Δ Γ t A ->
+--   Δ&Γ ⊢ t : X ->
+--   False
+-- | e, .var h, j => by grind
+-- | e, .app fn an, (.app fj aj) => fn.consistency_lemma e fj
+-- | e1, .tapp fn e2, (.tapp fj aj e3) => fn.consistency_lemma e1 fj
+-- | e, tn, .conv tj cv Bj => tn.consistency_lemma e tj
+
+-- theorem Typing.SnNor.consistency_lemma :
+--   Γ = [] ->
+--   C =t= (∀[★] t#0) ->
+--   SnNor T Δ Γ t A ->
+--   Δ&Γ ⊢ t : C ->
+--   False
+-- | e, cv, .tlam tn, (.tlam tj) => sorry
+-- | e, cv1, .tlam tn, (.conv tj cv2 Bj) => sorry
+-- | e, cv, .lam lr tn, tj => sorry
+-- -- | e, .tlam (.neu tn), .tlam tj => tn.consistency_lemma (by simp [e]) tj
+-- -- | e, .tlam (.red tr tn), .tlam tj => tn.consistency_lemma (by simp [e]) sorry
+-- | e, cv, .neu tn, j3 => tn.consistency_lemma e j3
+-- | e, cv, .red tr tn, j3 => tn.consistency_lemma e cv sorry
+
+-- theorem Typing.consistency : ¬ (Δ&[] ⊢ t : (∀[★] t#0))
+-- | j => SnNor.consistency_lemma rfl Conv.refl (j.fundamental $ SemSubst.id) (j |> cast (by simp))
+
+end TwoSortHet
